TouhouFormal/ECL.lean
@@ -15,4 +15,5 @@ import TouhouFormal.ECL.Assignment
 import TouhouFormal.ECL.Unary
 import TouhouFormal.ECL.FloatFunction
 import TouhouFormal.ECL.Random
+import TouhouFormal.ECL.Movement
 import TouhouFormal.ECL.Boss
